src/QUIC.Parse.VarInt.fsti
@@ -42,3 +42,31 @@ val read_varint: LL.leaf_reader parse_varint
 val jump_varint: LL.jumper parse_varint
 
 val serialize_varint_impl: LL.serializer32 serialize_varint
+
+module U32 = FStar.UInt32
+
+val validate_bounded_varint
+  (min: U32.t)
+  (max: U32.t { U32.v min <= U32.v max })
+: Tot (LL.validator (parse_bounded_varint (U32.v min) (U32.v max)))
+
+inline_for_extraction
+noextract
+val read_bounded_varint
+  (min: nat)
+  (max: nat { min <= max /\ max < 4294967296 })
+: Tot (LL.leaf_reader (parse_bounded_varint min max))
+
+inline_for_extraction
+noextract
+val jump_bounded_varint
+  (min: nat)
+  (max: nat { min <= max /\ max < 4294967296 })
+: Tot (LL.jumper (parse_bounded_varint min max))
+
+inline_for_extraction
+noextract
+val serialize_bounded_varint_impl
+  (min: nat)
+  (max: nat { min <= max /\ max < 4294967296 })
+: Tot (LL.serializer32 (serialize_bounded_varint min max))
